isabelle/examples/monads/set.thy
@@ -54,10 +54,10 @@ lemma "ap = \<Union>\<^sup>r \<circ> (image image)" unfolding all_defs by blast
 \<comment> \<open>...and so on\<close>
 
 text \<open>Check that applicative operations satisfy the corresponding laws.\<close>
-lemma applicative_unit1: "x = x \<ggreater> (unit \<^bold>I)" unfolding all_defs by simp
-lemma applicative_unit2: "(unit x) \<ggreater> (unit f) = unit (f x)" unfolding all_defs by simp
-lemma applicative_unit3: "(unit x) \<ggreater> f = f \<ggreater> unit (\<^bold>T x)" unfolding all_defs by simp
-lemma applicative_assoc: "(w \<ggreater> v) \<ggreater> u = w \<ggreater> (v \<ggreater> (u \<ggreater> (unit \<^bold>B)))" unfolding all_defs by fast
+lemma ap_identity:    "x \<ggreater> (unit \<^bold>I) = x" unfolding all_defs by simp
+lemma ap_composition: "w \<ggreater> (v \<ggreater> (u \<ggreater> (unit \<^bold>B))) = (w \<ggreater> v) \<ggreater> u" unfolding all_defs by fast
+lemma ap_homomorphism: "(unit x) \<ggreater> (unit f) = unit (f x)" unfolding all_defs by simp
+lemma ap_interchange: "(unit x) \<ggreater> f = f \<ggreater> unit (\<^bold>T x)" unfolding all_defs by simp
 
 
 subsection \<open>Monad\<close>
@@ -132,6 +132,9 @@ text \<open>Takes a monadic arrow and transforms it into an applicative arrow.\<
 abbreviation(input) intoArrowA::"('a \<Rightarrow> Set('b)) \<Rightarrow> Set('a \<Rightarrow> 'b)"
   where "intoArrowA \<equiv> intoFunSet"
 
+text \<open>Note that\<close>
+lemma "ap = bindr \<circ> intoArrowM" unfolding all_defs by fast
+
 
 subsubsection \<open>Functional composition\<close>
 
@@ -142,6 +145,12 @@ term "(;)  :: 'e-Env('a) \<Rightarrow> ('a \<Rightarrow> 'b) \<Rightarrow> 'e-En
 text \<open>Composition is associative and suitably interrelates with application to build pipelines.\<close>
 lemma "f ; (g ; h) = (f ; g) ; h" unfolding comb_defs ..
 lemma "(x |> f |> g |> h) = (x |> f ; g ; h)" unfolding comb_defs ..
+
+text \<open>Interrelation between application and composition.\<close>
+lemma "f ; g = (\<lambda>x. f x |> g)" unfolding comb_defs ..
+lemma "(\<circ>) = (\<lambda>g f x. g @ f @ x)" unfolding comb_defs ..
+lemma "(@) = (\<circ>) \<^bold>I" unfolding comb_defs ..
+lemma "(\<circ>) = \<^bold>D (@)" unfolding comb_defs ..
 
 
 subsubsection \<open>Monadic composition\<close>
@@ -165,6 +174,10 @@ term "(\<Zfinj>)  :: ('a \<Rightarrow> Set('b)) \<Rightarrow> ('b \<Rightarrow> 
 text \<open>As expected, monadic composition is associative and suitably interrelates with bind to build pipelines:\<close>
 lemma "f \<Zfinj> (g \<Zfinj> h) = (f \<Zfinj> g) \<Zfinj> h" unfolding all_defs by auto
 lemma "(x \<bind> f \<bind> g \<bind> h) = (x \<bind> f \<Zfinj> g \<Zfinj> h)" unfolding all_defs by auto
+
+text \<open>Bind in terms of monadic composition\<close>
+lemma "bindr = (\<Zfinj>) \<^bold>I" unfolding comb_defs ..
+lemma "(\<bind>) = (\<^bold>C \<circ> (\<Zfinj>)) \<^bold>I" unfolding comb_defs ..
 
 
 subsubsection \<open>Applicative composition\<close>
